test-suite/issues/issue390.v
@@ -1,0 +1,18 @@
+From Coq Require Import Lia NArith.NArith Program.Tactics.
+From Equations Require Export Equations.
+Ltac hidebody H ::= idtac.
+
+Import Pos N.
+Print Pos.compare.
+Open Scope N_scope.
+
+Instance lt_well_founded : WellFounded lt := Acc_intro_generator 100 lt_wf_0.
+
+(* Ltac Init.hidebody H ::= idtac. *)
+
+Equations? f (a : N) : N by wf a lt :=
+  f N0 := 0;
+  f (pos n) := succ (f (pred_N n)).
+Proof. lia. Qed.
+
+Compute f 42.
